# Topic 4 Exercises: Classification

Delia Walker-Jones

## 4.7.11
## 4.7.13
## 4.7.1
Prove that  
p(X) = e^(B~0~ + B~1~`*`X)/1 + e^(B~0~ + B~1~`*`X)  
is equivalent to  
p(X)/1 - p(X) = e^(B~0~ + B~1~`*`X)

p(X) `*` (1 + e^(B~0~ + B~1~`*`X)) = e^(B~0~ + B~1~`*`X)  
p(X) + (p(X) `*` e^(B~0~ + B~1~`*`X)) = e^(B~0~ + B~1~`*`X)
p(X) - e^(B~0~ + B~1~`*`X) = -(p(X) `*` e^(B~0~ + B~1~`*`X))  
e^(B~0~ + B~1~`*`X) = (p(X) `*` e^(B~0~ + B~1~`*`X)) - p(X)  
e^(B~0~ + B~1~`*`X) = p(X) `*` (e^(B~0~ + B~1~`*`X) - 1)  


## 4.7.8
The KNN (K = 1) approach 

## 4.7.9



